New definition for ifex_ite and ifex_bf2_rel

thy/BDT.thy
@@ -11,289 +11,108 @@ fun ifex_var_set :: "'a ifex \<Rightarrow> 'a set" where
   "ifex_var_set Trueif = {}" |
   "ifex_var_set Falseif = {}"
 
+fun ifex_top_var_set :: "'a ifex \<Rightarrow> 'a set" where
+  "ifex_top_var_set (IF v t e) = {v}" |
+  "ifex_top_var_set Trueif = {}" |
+  "ifex_top_var_set Falseif = {}"
+
 fun ifex_ordered :: "('a::linorder) ifex \<Rightarrow> bool" where
   "ifex_ordered (IF v t e) = ((\<forall>tv \<in> (ifex_var_set t \<union> ifex_var_set e). v < tv)
                        \<and> ifex_ordered t \<and> ifex_ordered e)" |
   "ifex_ordered Trueif = True" |
   "ifex_ordered Falseif = True"
 
-definition ifex_bf2_rel where
-  "ifex_bf2_rel = {(a,b). (\<forall>ass. a ass \<longleftrightarrow> val_ifex b ass) \<and> ifex_ordered b}"
+fun ifex_minimal :: "('a::linorder) ifex \<Rightarrow> bool" where
+  "ifex_minimal (IF v t e) = (t \<noteq> e \<and> ifex_minimal t \<and> ifex_minimal e)" |
+  "ifex_minimal Trueif = True" |
+  "ifex_minimal Falseif = True"
 
-lemma finite_ifex_var_set: "finite (ifex_var_set k)" by(induction k) simp_all
-lemma nonempty_if_var_set: "ifex_var_set (IF v t e) \<noteq> {}" by simp
-lemma ifex_ite_select_helper: "i = (IF iv it ie) \<Longrightarrow> k = (\<Union>(ifex_var_set ` {i,t,e})) \<Longrightarrow> finite k \<and> k \<noteq> {}"
-	using finite_ifex_var_set nonempty_if_var_set by auto
+definition ifex_bf2_rel where
+  "ifex_bf2_rel = {(a,b). (\<forall>ass. a ass \<longleftrightarrow> val_ifex b ass) \<and> ifex_ordered b \<and> ifex_minimal b}"
 
 fun restrict where
   "restrict (IF v t e) var val = (let rt = restrict t var val; re = restrict e var val in
                    (if v = var then (if val then rt else re) else (IF v rt re)))" |
   "restrict i _ _ = i"
 
-value "ifex_ordered (IF 1 Falseif (IF (0::nat) (IF 0 Falseif Falseif) Falseif))"
-value "restrict (IF (1::nat) Falseif (IF 0 (IF 0 Falseif Falseif) Falseif)) 1 False"
-(* definition "bf2_restrict (i::nat) (val::bool) (func::boolfunc2) \<equiv> (\<lambda>v. func (v(i:=val)))" *)
-value "ifex_ordered (IF (0::nat) (IF 0 Falseif Falseif) Falseif)"
-
-declare Let_def[simp]
-
-lemma not_element_restrict: "var \<notin> ifex_var_set (restrict b var val)"
-  by (induction b) auto
-
-lemma restrict_assignment: "val_ifex b (ass(var := val)) \<longleftrightarrow> val_ifex (restrict b var val) ass"
-  by (induction b) auto
-
-lemma restrict_variables_subset: "ifex_var_set (restrict b var val) \<subseteq> ifex_var_set b"
-  by (induction b) auto
-
-lemma restrict_ifex_ordered_invar: "ifex_ordered b \<Longrightarrow> ifex_ordered (restrict b var val)"
-  using restrict_variables_subset by (induction b) (fastforce)+
-
-lemma restrict_val_invar: "\<forall>ass. a ass = val_ifex b ass \<Longrightarrow> 
-      (bf2_restrict var val a) ass = val_ifex (restrict b var val) ass"
-  unfolding bf2_restrict_def using restrict_assignment by simp
-
-lemma restrict_ifex_bf2_rel:
-"(a, b) \<in> ifex_bf2_rel \<Longrightarrow> (bf2_restrict var val a, restrict b var val) \<in> ifex_bf2_rel"
-  unfolding ifex_bf2_rel_def using restrict_ifex_ordered_invar restrict_val_invar
-  by (clarsimp simp add: bf2_restrict_def restrict_assignment)
+fun restrict_top where
+  "restrict_top (IF v t e) var val =  (if v = var then (if val then t else e) else (IF v t e))" |
+  "restrict_top Trueif var val = Trueif" |
+  "restrict_top Falseif var val = Falseif"
 
 function ifex_ite :: "'a ifex \<Rightarrow> 'a ifex \<Rightarrow> 'a ifex \<Rightarrow> ('a :: linorder) ifex" where
   "ifex_ite Trueif t e = t" |
   "ifex_ite Falseif t e = e" |
-  "ifex_ite (IF iv it ie) t e = (let i = (IF iv it ie); x = select_lowest (\<Union>(ifex_var_set ` {i,t,e}));
-                                 l = ifex_ite (restrict i x True) (restrict t x True) (restrict e x True);
-                                 r = ifex_ite (restrict i x False) (restrict t x False) (restrict e x False) in 
+  "ifex_ite (IF iv it ie) t e =
+    (let i = (IF iv it ie); x = Min (\<Union>(ifex_top_var_set ` {i,t,e}));
+     l = ifex_ite (restrict_top i x True) (restrict_top t x True) (restrict_top e x True);
+     r = ifex_ite (restrict_top i x False) (restrict_top t x False) (restrict_top e x False) in
                         if l = r then l else IF x l r)"
 by pat_completeness auto
 
-lemma restrict_size_le: "size (restrict k x val) \<le> size k"
+declare Let_def[simp]
+
+lemma restrict_size_le: "size (restrict_top k x val) \<le> size k"
 by(induction k) (auto)
-lemma restrict_size_less: "x \<in> ifex_var_set k \<Longrightarrow> size (restrict k x val) < size k"
-proof(induction k)
-	case (IF v t e)
-	thus ?case
-	proof(cases "v = x")
-		case True
-		show ?thesis by(simp only: True restrict.simps refl if_True) (cases val, simp_all add: preorder_class.le_less_trans[OF restrict_size_le])
-	next
-		case False note of = this
-		show ?thesis
-		proof(cases "x \<in> ifex_var_set t")
-			case True
-			show ?thesis by(simp only: restrict.simps False if_False ifex.size) (simp add: IF.IH(1)[OF True] restrict_size_le add.commute add_le_less_mono)
-		next
-			case False
-			have *: "x \<in> ifex_var_set e"
-			proof(rule ccontr)
-				assume "x \<notin> ifex_var_set e"
-				note this False `v \<noteq> x`
-				with IF.prems show False by simp
-			qed
-			show ?thesis by(simp only: restrict.simps of if_False ifex.size) (simp add: IF.IH(2)[OF *] add_mono_thms_linordered_field(4) restrict_size_le)
-		qed
-	qed
-qed simp_all
-lemma restrict_size_eqE: "size k = size (restrict k x val) \<Longrightarrow> x \<notin> ifex_var_set k"
-	using less_not_refl restrict_size_less by metis
 
-lemma termlemma2: "xa = select_lowest (\<Union>(ifex_var_set ` {(IF iv it ie), t, e})) \<Longrightarrow>
-       (size (restrict (IF iv it ie) xa val) + size (restrict t xa val) + size (restrict e xa val)) < (size (IF iv it ie) + size t + size e)"
-proof(rule ccontr, unfold not_less)
-	case goal1 thus ?case
-	proof(cases "size (IF iv it ie) + size t + size e < size (restrict (IF iv it ie) xa val) + size (restrict t xa val) + size (restrict e xa val)")
-		case False
-		with goal1 have *: "size (IF iv it ie) + size t + size e = size (restrict (IF iv it ie) xa val) + size (restrict t xa val) + size (restrict e xa val)" by auto
-		have 1: "size (IF iv it ie) = size (restrict (IF iv it ie) xa val)" using restrict_size_le * by (metis False add_less_le_mono order.not_eq_order_implies_strict)
-		have 2: "size t = size (restrict t xa val)" using restrict_size_le * by (metis False add.commute add_less_le_mono order.not_eq_order_implies_strict)
-		have 3: "size e = size (restrict e xa val)" using * 1 2 by linarith
-		note restrict_size_eqE[OF 1] restrict_size_eqE[OF 2] restrict_size_eqE[OF 3]
-		then show False unfolding goal1 using ifex_ite_select_helper[OF refl refl] 
-			conjunct1[OF select_is_lowest[unfolded is_lowest_element_def], of "(\<Union>(ifex_var_set ` {(IF iv it ie), t, e}))"] by auto 
-	next
-		case True thus False using restrict_size_le by (metis add_mono_thms_linordered_semiring(1) leD)
-	qed
-qed
-lemma termlemma: "xa = select_lowest (\<Union>(ifex_var_set ` {(IF iv it ie), t, e})) \<Longrightarrow>
-       (case (restrict (IF iv it ie) xa val, restrict t xa val, restrict e xa val) of (i, t, e) \<Rightarrow> size i + size t + size e) < (case (IF iv it ie, t, e) of (i, t, e) \<Rightarrow> size i + size t + size e)"
-using termlemma2 by fast
-termination ifex_ite by(relation "measure (\<lambda>(i,t,e). size i + size t + size e)", rule wf_measure, unfold in_measure) (simp_all only: termlemma)+
+lemma restrict_size_element: "var \<in> ifex_top_var_set k \<Longrightarrow>
+                                   size (restrict_top k var val) < size k"
+by(induction k) (auto)
 
-lemma restrict_untouched_id: "x \<notin> ifex_var_set t \<Longrightarrow> restrict t x val = t" (* umkehrung gilt auch\<dots> *)
-proof(induction t)
-	case (IF v t e)
-	from IF.prems have "x \<notin> ifex_var_set t" "x \<notin> ifex_var_set e" by auto
-	note mIH = IF.IH(1)[OF this(1)] IF.IH(2)[OF this(2)]
-	from IF.prems have "x \<noteq> v" by simp
-	thus ?case unfolding restrict.simps Let_def mIH  by simp
-qed simp_all
+lemma ifex_top_var_set_finite: "finite (ifex_top_var_set k)"
+  by (induction k) auto
 
-(* INDUCTIVE DEFINITION *)
-
-abbreviation ifex_variables_ite where 
-  "ifex_variables_ite i t e \<equiv> 
-   ifex_var_set i \<union> ifex_var_set t \<union> ifex_var_set e"
-
-inductive ind_ite :: "('a::linorder) ifex \<Rightarrow> 'a ifex \<Rightarrow> 'a ifex \<Rightarrow> 'a ifex \<Rightarrow> bool" where
-ind_ite_true:   "ind_ite t Trueif t e" |
-ind_ite_false:  "ind_ite e Falseif t e" |
-ind_ite_if:     "x \<in> ifex_variables_ite i t e \<Longrightarrow>
-   \<forall>v \<in> ifex_variables_ite i t e. x \<le> v \<Longrightarrow>
-   i = IF iv tifex eifex \<Longrightarrow>
-   ind_ite l (restrict i x True) (restrict t x True) (restrict e x True) \<Longrightarrow>
-   ind_ite r (restrict i x False) (restrict t x False) (restrict e x False) \<Longrightarrow>
-   ind_ite (if l = r then l else IF x l r) i t e"
-
-lemma ifex_var_set_union_image_equi:
-  "\<Union>(ifex_var_set ` {i,t,e}) =
-   ifex_var_set i \<union> ifex_var_set t \<union> ifex_var_set e"
-  by blast
-
-lemma ifex_ite_ind_ite_equi: "ifex_ite i t e = b \<longleftrightarrow> ind_ite b i t e"
-proof(rule iffI)
-assume "ifex_ite i t e = b" thus "ind_ite b i t e"
-proof(induct arbitrary: b rule: ifex_ite.induct)
-  case("3" iv tifex eifex t e) note ifex_ite_IF = "3"
-  obtain i y l r 
-    where i_def: "i = IF iv tifex eifex" and
-          y_def: "y = select_lowest (\<Union>(ifex_var_set ` {i,t,e}))" and
-          r_def: "r = ifex_ite (restrict i y False) (restrict t y False) (restrict e y False)" and
-          l_def: "l = ifex_ite (restrict i y True) (restrict t y True) (restrict e y True)" by simp
-  from i_def have "finite (ifex_variables_ite i t e)" "ifex_variables_ite i t e \<noteq> {}"
-    by (simp_all add: finite_ifex_var_set)
-  from select_is_lowest[OF this(1) this(2)] y_def
-    have smallest: "y \<in> ifex_variables_ite i t e" "\<forall>v \<in> ifex_variables_ite i t e. y \<le> v"
-    unfolding is_lowest_element_def by (simp_all only: ifex_var_set_union_image_equi) (simp)
-  from l_def r_def i_def y_def ifex_ite_IF(1)[of i y l] ifex_ite_IF(2)[of i y l r] 
-    have landr: "ind_ite l (restrict i y True) (restrict t y True) (restrict e y True)"
-                "ind_ite r (restrict i y False) (restrict t y False) (restrict e y False)" by auto
-  from ifex_ite_IF(3) l_def r_def y_def i_def have "b = (if l = r then l else IF y l r)" by force
-  with ind_ite_if[OF smallest i_def landr] show ?case using i_def by simp
-qed (auto simp add: ind_ite.intros)
-next
-assume "ind_ite b i t e" thus "ifex_ite i t e = b"
-proof(induction rule: ind_ite.induct)
-  case(ind_ite_if x i t e iv tifex eifex l r)
-    from this(3) have "ifex_variables_ite i t e \<noteq> {}" "finite (ifex_variables_ite i t e)"
-      using finite_ifex_var_set by auto
-    from select_is_lowest[OF this(2) this(1)] ind_ite_if(1,2,3)
-      have "select_lowest (\<Union>(ifex_var_set ` {IF iv tifex eifex, t, e})) = x"
-      unfolding is_lowest_element_def by (subst ifex_var_set_union_image_equi) force
-    from this ind_ite_if(3,6,7) show ?case by simp
-qed (auto)
-qed
-
-lemma ind_ite_variables_subset: "ind_ite b i t e \<Longrightarrow> 
-  ifex_var_set b \<subseteq> ifex_var_set i \<union> ifex_var_set t \<union> ifex_var_set e"
-proof(induction rule: ind_ite.induct)
-  case(ind_ite_if x i t e iv tv ev l r) 
-    from this(6,7) restrict_variables_subset[of _ x _] have 
-         "ifex_var_set l \<subseteq> ifex_variables_ite i t e"
-         "ifex_var_set r \<subseteq> ifex_variables_ite i t e"
-        by (blast)+
-     with ind_ite_if(1) show ?case by simp
-qed (auto)
-
-lemma ind_ite_not_element: "ind_ite b i t e \<Longrightarrow> x \<notin> ifex_variables_ite i t e  \<Longrightarrow>
-                            x \<notin> ifex_var_set b"
-proof(induction arbitrary: x rule: ind_ite.induct)
-  case(ind_ite_if y i t e iv tv ev l r) 
-    from this(1,8) this(6)[of x] this(7)[of x]
-    have "x \<noteq> y" "x \<notin> ifex_var_set l" "x \<notin> ifex_var_set r"
-      using restrict_variables_subset contra_subsetD by (fastforce)+
-    thus ?case by simp
-qed (auto)
-
-lemma ind_ite_ifex_ordered: "ind_ite b i t e \<Longrightarrow> 
-                             ifex_ordered i \<Longrightarrow> ifex_ordered t \<Longrightarrow> ifex_ordered e \<Longrightarrow> 
-                             ifex_ordered b"
-proof(induction rule: ind_ite.induct)
-  case(ind_ite_if x i t e iv tv ev l r) from this(6,7,8,9,10) 
-    have 0: "ifex_ordered l" "ifex_ordered r" 
-    using restrict_ifex_ordered_invar by auto
-  from ind_ite_if(4,5) have 1:"x \<notin> ifex_var_set l" "x \<notin> ifex_var_set r" 
-     using ind_ite_not_element not_element_restrict by fastforce+
-  from ind_ite_if(2) ind_ite_variables_subset[OF ind_ite_if(4)]
-    have 2: "\<forall>y \<in> ifex_var_set l. x \<le> y" using restrict_variables_subset by fast
-  from ind_ite_if(2) ind_ite_variables_subset[OF ind_ite_if(5)]
-    have 3: "\<forall>y \<in> ifex_var_set r. x \<le> y" using restrict_variables_subset by fast
-  from 0 1 2 3 show ?case using le_neq_trans by fastforce
-qed (simp)
-
-lemma bf_ite_assignment_invar:
-  "ass y = x \<Longrightarrow> bf_ite ia ta ea ass = bf_ite (bf2_restrict y x ia) (bf2_restrict y x ta) 
-                                              (bf2_restrict y x ea) ass"
-  unfolding bf_ite_def bf2_restrict_def by force
-
-lemma ind_ite_val_invar: "ind_ite b ib tb eb \<Longrightarrow>
-  \<forall>ass. ia ass = val_ifex ib ass \<Longrightarrow>
-  \<forall>ass. ta ass = val_ifex tb ass \<Longrightarrow>
-  \<forall>ass. ea ass = val_ifex eb ass \<Longrightarrow>
-  \<forall>ass. (bf_ite ia ta ea) ass = val_ifex b ass"
-proof(induction arbitrary: ia ta ea rule: ind_ite.induct)
-  case(ind_ite_if y i t e iv tv ev l r)
-  note rvi_mult = restrict_val_invar[OF ind_ite_if(8)]
-                  restrict_val_invar[OF ind_ite_if(9)]
-                  restrict_val_invar[OF ind_ite_if(10)]
-  from ind_ite_if(6) ind_ite_if(7) rvi_mult bf_ite_assignment_invar[of _ y _ ia ta ea]
-    have "\<forall>ass. bf_ite (bf2_restrict y True ia) (bf2_restrict y True ta)
-                       (bf2_restrict y True ea) ass
-                 = val_ifex l ass" 
-         "\<forall>ass. bf_ite (bf2_restrict y False ia) (bf2_restrict y False ta)
-                       (bf2_restrict y False ea) ass
-                = val_ifex r ass"
-         "\<And>ass. ass y \<Longrightarrow> bf_ite ia ta ea ass =
-                           bf_ite (bf2_restrict y True ia) (bf2_restrict y True ta)
-                                  (bf2_restrict y True ea) ass"
-         "\<And>ass. \<not> ass y \<Longrightarrow> bf_ite ia ta ea ass =
-                             bf_ite (bf2_restrict y False ia) (bf2_restrict y False ta) 
-                                    (bf2_restrict y False ea) ass"
-       by fastforce+
-  thus ?case by force
-qed (auto simp add: bf_ite_def)
-
-lemma "ind_ite b ib tb eb \<Longrightarrow>
-       (ia, ib) \<in> ifex_bf2_rel \<Longrightarrow>
-       (ta, tb) \<in> ifex_bf2_rel \<Longrightarrow>
-       (ea, eb) \<in> ifex_bf2_rel \<Longrightarrow>
-       (bf_ite ia ta ea, b) \<in> ifex_bf2_rel"
-  unfolding ifex_bf2_rel_def by (simp add: ind_ite_ifex_ordered ind_ite_val_invar)
-
-fun ifex_minimal :: "'a ifex \<Rightarrow> bool" where
-  "ifex_minimal (IF v t e) = ((t \<noteq> e) & ifex_minimal t & ifex_minimal e)" |
-  "ifex_minimal Trueif = True" |
-  "ifex_minimal Falseif = True"
-
-lemma ifex_ordered_restrict_branches:
-  "ifex_ordered (IF x l r) \<Longrightarrow> restrict (IF x l r) x val = (if val then l else r)"
-  using restrict_untouched_id by fastforce
-
-lemma ifex_minimal_restrict_invar:
-       "ifex_ordered i \<Longrightarrow> ifex_minimal i \<Longrightarrow> \<forall>v \<in> ifex_var_set i. var \<le> v \<Longrightarrow>
-       ifex_minimal (restrict i var val)"
-proof(induction i)
-case (IF x i1 i2) show ?case
-proof(cases "var \<in> ifex_var_set (IF x i1 i2)")
-  case False 
-    with restrict_untouched_id have "(restrict (IF x i1 i2) var val) = (IF x i1 i2)" by fast
-    with IF(4) show ?thesis by simp
+lemma termlemma2:
+  assumes "var = Min (\<Union>(ifex_top_var_set ` {(IF iv it ie), t, e}))"
+  shows
+  "(size (restrict_top (IF iv it ie) var val) +
+    size (restrict_top t var val) +
+    size (restrict_top e var val))
+    < (size (IF iv it ie) + size t + size e)"
+proof -
+  from assms have "(\<Union>(ifex_top_var_set ` {(IF iv it ie), t, e})) \<noteq> {}"
+                  "finite (\<Union>(ifex_top_var_set ` {(IF iv it ie), t, e}))"
+    using ifex_top_var_set_finite by fastforce+
+  from Min_in[OF this(2) this(1)] assms have "var \<in> (\<Union>(ifex_top_var_set ` {(IF iv it ie), t, e}))"
+    by fast
+  from this have var_elem: "var \<in> ifex_top_var_set (IF iv it ie) \<or>
+                            var \<in> ifex_top_var_set t \<or>
+                            var \<in> ifex_top_var_set e"
+    by blast
+  from this show ?thesis
+proof(rule disjE)
+  case goal1 then have
+    "size (restrict_top (IF iv it ie) var val) < size (IF iv it ie)"
+    "size (restrict_top t var val) + size (restrict_top e var val) \<le> size t + size e"
+    by(simp add: restrict_size_le add_le_mono)+
+  from this show ?thesis by linarith
   next
-  case True
-    with IF(3,5) have "var = x" apply(auto) using not_less by auto
-    with IF(3,4) show ?thesis using ifex_ordered_restrict_branches by fastforce
+  case goal2 then show ?thesis
+  proof(rule disjE)
+    case goal1 then have 0: "size (restrict_top t var val) < size t"
+        using restrict_size_element by fastforce
+      have "size (restrict_top (IF iv it ie) var val) + size (restrict_top e var val) \<le>
+            size (IF iv it ie) + size e" by (meson restrict_size_le add_le_mono)
+      with 0 show ?thesis by linarith
+    next
+    case goal2 then have 0: "size (restrict_top e var val) < size e"
+        using restrict_size_element by fastforce
+      have "size (restrict_top (IF iv it ie) var val) + size (restrict_top t var val) \<le>
+            size (IF iv it ie) + size t" by (meson restrict_size_le add_le_mono)
+      with 0 show ?thesis by linarith
+    qed
   qed
-qed (auto)
+qed
 
-lemma ind_ite_minimal:
-  "ind_ite b ib tb eb \<Longrightarrow> ifex_ordered ib \<Longrightarrow> ifex_ordered tb \<Longrightarrow> ifex_ordered eb \<Longrightarrow>
-   ifex_minimal ib \<Longrightarrow> ifex_minimal tb \<Longrightarrow> ifex_minimal eb \<Longrightarrow>
-   ifex_minimal b"
-proof(induction rule: ind_ite.induct)
-  case(ind_ite_if x i t e iv tifex eifex l r) 
-    then have lr_minimal: "ifex_minimal l" "ifex_minimal r"
-      using restrict_ifex_ordered_invar ifex_minimal_restrict_invar by(blast)+
-    thus ?case by simp
-qed (simp)
+lemma termlemma: "xa = Min (\<Union>(ifex_top_var_set ` {(IF iv it ie), t, e})) \<Longrightarrow>
+       (case (restrict_top (IF iv it ie) xa val, restrict_top t xa val, restrict_top e xa val)
+             of (i, t, e) \<Rightarrow> size i + size t + size e) < (case (IF iv it ie, t, e)
+             of (i, t, e) \<Rightarrow> size i + size t + size e)"
+using termlemma2 by fast
+
+termination ifex_ite
+  by (relation "measure (\<lambda>(i,t,e). size i + size t + size e)", rule wf_measure, unfold in_measure)
+     (simp_all only: termlemma)+
 
 
 end
